Basic Scheduler library that hides all state inside a nullary abstract predicate

platform/tests/BabyThreadDriver.v
@@ -1,12 +1,26 @@
 Require Import Thread0 BabyThread Bootstrap.
 
 
-Section boot.
+Module Type S.
   Variable heapSize : nat.
+End S.
 
+Module Make(M : S).
+Import M.
+
+Module M'.
+  Definition globalSched : W := (heapSize + 50) * 4.
+End M'.
+
+Import M'.
+
+Module E := BabyThread.Make(M').
+Import E.
+
+Section boot.
   Hypothesis heapSizeLowerBound : (3 <= heapSize)%nat.
 
-  Definition size := heapSize + 50.
+  Definition size := heapSize + 50 + 1.
 
   Hypothesis mem_size : goodSize (size * 4)%nat.
 
@@ -14,33 +28,33 @@ Section boot.
     goodSize.
   Qed.
 
-  Definition bootS := bootS heapSize.
+  Definition bootS := bootS heapSize 1.
 
-  Definition boot := bimport [[ "malloc"!"init" @ [Malloc.initS], "test"!"main" @ [BabyThread.mainS] ]]
+  Definition boot := bimport [[ "malloc"!"init" @ [Malloc.initS], "test"!"main" @ [E.mainS] ]]
     bmodule "main" {{
       bfunctionNoRet "main"() [bootS]
         Sp <- (heapSize * 4)%nat;;
 
-        Assert [PREonly[_] 0 =?> heapSize];;
+        Assert [PREonly[_] globalSched =?> 1 * 0 =?> heapSize];;
 
         Call "malloc"!"init"(0, heapSize)
-        [PREonly[_] mallocHeap 0];;
+        [PREonly[_] globalSched =?> 1 * mallocHeap 0];;
 
         Call "test"!"main"()
-        [PREonly[_] [| False |] ];;
-
-        Fail
+        [PREonly[_] [| False |] ]
       end
     }}.
 
   Theorem ok : moduleOk boot.
-    vcgen; abstract (sep genesisHints; eauto).
+    vcgen; abstract (unfold globalSched; genesis).
   Qed.
 
   Definition m0 := link Malloc.m boot.
   Definition m1 := link Queue.m m0.
-  Definition m2 := link Q.m m1.
-  Definition m3 := link BabyThread.m m2.
+  Definition m2 := link E.T.T.Q''.m m1.
+  Definition m3 := link E.T.T.Q''.Q'.m m2.
+  Definition m4 := link E.T.T.Q''.Q'.Q.m m3.
+  Definition m5 := link E.m m4.
 
   Lemma ok0 : moduleOk m0.
     link Malloc.ok ok.
@@ -51,11 +65,19 @@ Section boot.
   Qed.
 
   Lemma ok2 : moduleOk m2.
-    link Q.ok ok1.
+    link E.T.T.Q''.ok ok1.
   Qed.
 
   Lemma ok3 : moduleOk m3.
-    link BabyThread.ok ok2.
+    link E.T.T.Q''.Q'.ok ok2.
+  Qed.
+
+  Lemma ok4 : moduleOk m4.
+    link E.T.T.Q''.Q'.Q.ok ok3.
+  Qed.
+
+  Lemma ok5 : moduleOk m5.
+    link E.ok ok4.
   Qed.
 
   Variable stn : settings.
@@ -66,7 +88,7 @@ Section boot.
     -> l1 = l2.
 
   Hypothesis agree : forall l pre bl,
-    LabelMap.MapsTo l (pre, bl) (XCAP.Blocks m3)
+    LabelMap.MapsTo l (pre, bl) (XCAP.Blocks m5)
     -> exists w, Labels stn l = Some w
       /\ prog w = Some bl.
 
@@ -79,6 +101,8 @@ Section boot.
   Hypothesis mem_high : forall w, $(size * 4) <= w -> st.(Mem) w = None.
 
   Theorem safe : safe stn prog (w, st).
-    safety ok3.
+    safety ok5.
   Qed.
 End boot.
+
+End Make.
