platform/tests/SharedList.v
@@ -1,40 +1,47 @@
 Require Import Thread SinglyLinkedList.
 
 
-Parameter globalList : W.
+Module Type S.
+  Variables globalList globalSched : W.
+End S.
 
-Module M.
+Module Make(M : S).
+Import M.
+
+Module M'''.
+  Definition globalSched := M.globalSched.
+
   Open Scope Sep_scope.
 
-  Definition realInv : HProp := Ex p, globalList =*> p * Ex ls, sll ls p.
+  Definition globalInv : HProp := Ex p, globalList =*> p * Ex ls, sll ls p.
+End M'''.
 
-  Definition globalInv (_ : W) : hpropB ((settings * state : Type)%type :: nil) :=
-    ^[realInv].
-End M.
+Ltac unf := unfold M'''.globalSched, M'''.globalInv in *.
 
-Module T := Make(M).
-Import M T.
+Module T := Thread.Make(M''').
 
-Ltac sep := T.sep ltac:(unfold globalInv, realInv in *) SinglyLinkedList.hints.
+Import T M'''.
+Export T M'''.
 
+Ltac sep := T.sep unf SinglyLinkedList.hints.
 
-Definition handlerS := SPEC("sc") reserving 24
-  PREonly[V] tq (V "sc") * realInv * mallocHeap 0.
+Definition handlerS := SPEC reserving 29
+  PREonly[_] sched * globalInv * mallocHeap 0.
 
-Definition mainS := SPEC reserving 23
-  PREonly[_] globalList =?> 1 * mallocHeap 0.
+Definition mainS := SPEC reserving 36
+  PREonly[_] globalSched =?> 1 * globalList =?> 1 * mallocHeap 0.
 
 Definition m := bimport [[ "malloc"!"malloc" @ [mallocS], "malloc"!"free" @ [freeS],
-                           "threadq"!"init" @ [initS], "threadq"!"exit" @ [exitS],
-                           "threadq"!"spawn" @ [spawnS], "threadq"!"yield" @ [yieldS] ]]
+                           "scheduler"!"init" @ [initS], "scheduler"!"exit" @ [exitS],
+                           "scheduler"!"spawn" @ [spawnS], "scheduler"!"yield" @ [yieldS] ]]
   bmodule "test" {{
-    bfunctionNoRet "handler"("sc", "i", "p", "r") [handlerS]
+    bfunctionNoRet "handler"("i", "p", "r") [handlerS]
       "i" <- 0;; (* Loop counter *)
 
-      [PREonly[V] tq (V "sc") * realInv * mallocHeap 0]
+      [PREonly[_] sched * globalInv * mallocHeap 0]
       While ("i" < 10) {
         "r" <-- Call "malloc"!"malloc"(0, 2)
-        [PREonly[V, R] [| R <> 0 |] * [| freeable R 2 |] * R =?> 2 * tq (V "sc") * realInv * mallocHeap 0];;
+        [PREonly[V, R] [| R <> 0 |] * [| freeable R 2 |] * R =?> 2 * sched * globalInv * mallocHeap 0];;
 
         "r" *<- "i";;
         "p" <-* globalList;;
@@ -43,20 +50,20 @@ Definition m := bimport [[ "malloc"!"malloc" @ [mallocS], "malloc"!"free" @ [fre
         "i" <- "i" + 1;;
 
         Yield
-        [PREonly[V] tq (V "sc") * realInv * mallocHeap 0]
+        [PREonly[_] sched * globalInv * mallocHeap 0]
       };;
 
       "p" <-* globalList;;
-      [PREonly[V] tq (V "sc") * globalList =*> V "p" * Ex ls, sll ls (V "p") * mallocHeap 0]
+      [PREonly[V] sched * globalList =*> V "p" * Ex ls, sll ls (V "p") * mallocHeap 0]
       While ("p" <> 0) {
         "r" <- "p";;
         "p" <-* "p" + 4;;
         globalList *<- "p";;
         Call "malloc"!"free"(0, "r", 2)
-        [PREonly[V] tq (V "sc") * realInv * mallocHeap 0];;
+        [PREonly[_] sched * globalInv * mallocHeap 0];;
 
         Yield
-        [PREonly[V] tq (V "sc") * realInv * mallocHeap 0];;
+        [PREonly[_] sched * globalInv * mallocHeap 0];;
 
         "p" <-* globalList
       };;
@@ -65,14 +72,14 @@ Definition m := bimport [[ "malloc"!"malloc" @ [mallocS], "malloc"!"free" @ [fre
     end with bfunctionNoRet "main"("sc") [mainS]
       globalList *<- 0;;
 
-      "sc" <-- Call "threadq"!"init"()
-      [PREonly[_, R] tq R * realInv * mallocHeap 0];;
+      Init
+      [PREonly[_] sched * globalInv * mallocHeap 0];;
 
-      Spawn("test"!"handler", 26)
-      [PREonly[V] tq (V "sc") * realInv * mallocHeap 0];;
+      Spawn("test"!"handler", 30)
+      [PREonly[_] sched * globalInv * mallocHeap 0];;
 
-      Spawn("test"!"handler", 26)
-      [PREonly[V] tq (V "sc") * realInv * mallocHeap 0];;
+      Spawn("test"!"handler", 30)
+      [PREonly[_] sched * globalInv * mallocHeap 0];;
 
       Go
     end
@@ -81,3 +88,5 @@ Definition m := bimport [[ "malloc"!"malloc" @ [mallocS], "malloc"!"free" @ [fre
 Theorem ok : moduleOk m.
   vcgen; abstract sep.
 Qed.
+
+End Make.
