platform/tests/SharedListDriver.v
@@ -1,4 +1,4 @@
-Require Import Thread0 ListBuilder Bootstrap.
+Require Import Thread0 SharedList Bootstrap.
 
 
 Module Type S.
@@ -10,17 +10,18 @@ Import M.
 
 Module M'.
   Definition globalSched : W := (heapSize + 50) * 4.
+  Definition globalList : W := globalSched ^+ $4.
 End M'.
 
 Import M'.
 
-Module E := ListBuilder.Make(M').
+Module E := SharedList.Make(M').
 Import E.
 
 Section boot.
   Hypothesis heapSizeLowerBound : (3 <= heapSize)%nat.
 
-  Definition size := heapSize + 50 + 1.
+  Definition size := heapSize + 50 + 2.
 
   Hypothesis mem_size : goodSize (size * 4)%nat.
 
@@ -28,17 +29,17 @@ Section boot.
     goodSize.
   Qed.
 
-  Definition bootS := bootS heapSize 1.
+  Definition bootS := bootS heapSize 2.
 
   Definition boot := bimport [[ "malloc"!"init" @ [Malloc.initS], "test"!"main" @ [E.mainS] ]]
     bmodule "main" {{
       bfunctionNoRet "main"() [bootS]
         Sp <- (heapSize * 4)%nat;;
 
-        Assert [PREonly[_] globalSched =?> 1 * 0 =?> heapSize];;
+        Assert [PREonly[_] globalSched =?> 2 * 0 =?> heapSize];;
 
         Call "malloc"!"init"(0, heapSize)
-        [PREonly[_] globalSched =?> 1 * mallocHeap 0];;
+        [PREonly[_] globalList =?> 1 * globalSched =?> 1 * mallocHeap 0];;
 
         Call "test"!"main"()
         [PREonly[_] [| False |] ]
@@ -46,14 +47,14 @@ Section boot.
     }}.
 
   Theorem ok : moduleOk boot.
-    vcgen; abstract (unfold globalSched; genesis).
+    vcgen; abstract (unfold globalSched, M'.globalList, M'.globalSched; genesis).
   Qed.
 
   Definition m0 := link Malloc.m boot.
   Definition m1 := link Queue.m m0.
-  Definition m2 := link E.T.T.Q''.m m1.
-  Definition m3 := link E.T.T.Q''.Q'.m m2.
-  Definition m4 := link E.T.T.Q''.Q'.Q.m m3.
+  Definition m2 := link E.T.Q''.m m1.
+  Definition m3 := link E.T.Q''.Q'.m m2.
+  Definition m4 := link E.T.Q''.Q'.Q.m m3.
   Definition m5 := link E.m m4.
 
   Lemma ok0 : moduleOk m0.
@@ -65,15 +66,15 @@ Section boot.
   Qed.
 
   Lemma ok2 : moduleOk m2.
-    link E.T.T.Q''.ok ok1.
+    link E.T.Q''.ok ok1.
   Qed.
 
   Lemma ok3 : moduleOk m3.
-    link E.T.T.Q''.Q'.ok ok2.
+    link E.T.Q''.Q'.ok ok2.
   Qed.
 
   Lemma ok4 : moduleOk m4.
-    link E.T.T.Q''.Q'.Q.ok ok3.
+    link E.T.Q''.Q'.Q.ok ok3.
   Qed.
 
   Lemma ok5 : moduleOk m5.
