examples/comparison/Combined.v
@@ -13,4 +13,5 @@ Qed.
 
 Require Import AMD64_gas.
 
+Set Printing Depth 999999.
 Eval compute in moduleS program.
