platform/tests/SharedListAMD64.v
@@ -1,4 +1,4 @@
-Require Import Bedrock ListBuilderDriver AMD64_gas.
+Require Import Bedrock SharedListDriver AMD64_gas.
 
 Module M.
   Definition heapSize := 1024.
