platform/tests/Spawn.v
@@ -1,25 +1,31 @@
 Require Import Thread0.
 
 
-Definition handlerS := SPEC("sc") reserving 24
-  PREonly[V] sched (V "sc") * mallocHeap 0.
+Module Make(M : S).
+Import M.
 
-Definition mainS := SPEC reserving 23
-  PREonly[_] mallocHeap 0.
+Module T := Thread0.Make(M).
+Import T.
 
-Definition m := bimport [[ "threadq"!"init" @ [initS], "threadq"!"exit" @ [exitS],
-                           "threadq"!"spawn" @ [spawnS] ]]
+Definition handlerS := SPEC reserving 36
+  PREonly[_] sched * mallocHeap 0.
+
+Definition mainS := SPEC reserving 36
+  PREonly[_] globalSched =?> 1 * mallocHeap 0.
+
+Definition m := bimport [[ "scheduler"!"init" @ [initS], "scheduler"!"exit" @ [exitS],
+                           "scheduler"!"spawn" @ [spawnS] ]]
   bmodule "test" {{
-    bfunctionNoRet "handler"("sc") [handlerS]
-      Spawn("test"!"handler", 26)
-      [PREonly[V] sched (V "sc") * mallocHeap 0];;
+    bfunctionNoRet "handler"() [handlerS]
+      Spawn("test"!"handler", 37)
+      [PREonly[_] sched * mallocHeap 0];;
       Exit
-    end with bfunctionNoRet "main"("sc") [mainS]
-      "sc" <-- Call "threadq"!"init"()
-      [PREonly[_, R] sched R * mallocHeap 0];;
+    end with bfunctionNoRet "main"() [mainS]
+      Init
+      [PREonly[_] sched * mallocHeap 0];;
 
-      Spawn("test"!"handler", 26)
-      [PREonly[V] sched (V "sc") * mallocHeap 0];;
+      Spawn("test"!"handler", 37)
+      [PREonly[_] sched * mallocHeap 0];;
 
       Go
     end
@@ -28,3 +34,5 @@ Definition m := bimport [[ "threadq"!"init" @ [initS], "threadq"!"exit" @ [exitS
 Theorem ok : moduleOk m.
   vcgen; abstract sep_auto.
 Qed.
+
+End Make.
